Flapjack.lean
@@ -14,6 +14,7 @@ import Flapjack.Semantics
 import Flapjack.PanValues
 import Flapjack.PanMemory
 import Flapjack.RiscV.Model
+import Flapjack.RiscV.PanMemory
 import Flapjack.RiscV.PanSemantics
 import Flapjack.RiscV.Backend
 import Flapjack.RiscV.Calls
